program_logic/viewshifts.v
@@ -24,7 +24,7 @@ Implicit Types P Q R : iProp Λ Σ.
 Lemma vs_alt E1 E2 P Q : (P ⊑ pvs E1 E2 Q) → P ={E1,E2}=> Q.
 Proof.
   intros; rewrite -{1}always_const; apply always_intro, impl_intro_l.
-  by rewrite always_const (right_id _ _).
+  by rewrite always_const right_id.
 Qed.
 
 Global Instance vs_ne E1 E2 n :
@@ -51,7 +51,7 @@ Lemma vs_transitive E1 E2 E3 P Q R :
   E2 ⊆ E1 ∪ E3 → ((P ={E1,E2}=> Q) ∧ (Q ={E2,E3}=> R)) ⊑ (P ={E1,E3}=> R).
 Proof.
   intros; rewrite -always_and; apply always_intro, impl_intro_l.
-  rewrite always_and (associative _) (always_elim (P → _)) impl_elim_r.
+  rewrite always_and assoc (always_elim (P → _)) impl_elim_r.
   by rewrite pvs_impl_r; apply pvs_trans.
 Qed.
 
@@ -69,12 +69,12 @@ Qed.
 Lemma vs_frame_l E1 E2 P Q R : (P ={E1,E2}=> Q) ⊑ (R ★ P ={E1,E2}=> R ★ Q).
 Proof.
   apply always_intro, impl_intro_l.
-  rewrite -pvs_frame_l always_and_sep_r -always_wand_impl -(associative _).
+  rewrite -pvs_frame_l always_and_sep_r -always_wand_impl -assoc.
   by rewrite always_elim wand_elim_r.
 Qed.
 
 Lemma vs_frame_r E1 E2 P Q R : (P ={E1,E2}=> Q) ⊑ (P ★ R ={E1,E2}=> Q ★ R).
-Proof. rewrite !(commutative _ _ R); apply vs_frame_l. Qed.
+Proof. rewrite !(comm _ _ R); apply vs_frame_l. Qed.
 
 Lemma vs_mask_frame E1 E2 Ef P Q :
   Ef ∩ (E1 ∪ E2) = ∅ → (P ={E1,E2}=> Q) ⊑ (P ={E1 ∪ Ef,E2 ∪ Ef}=> Q).
@@ -91,11 +91,11 @@ Lemma vs_open_close N E P Q R :
   (inv N R ★ (▷ R ★ P ={E ∖ nclose N}=> ▷ R ★ Q)) ⊑ (P ={E}=> Q).
 Proof.
   intros; apply (always_intro' _ _), impl_intro_l.
-  rewrite always_and_sep_r' associative [(P ★ _)%I]commutative -associative.
+  rewrite always_and_sep_r' assoc [(P ★ _)%I]comm -assoc.
   rewrite -(pvs_open_close E N) //. apply sep_mono; first done.
   apply wand_intro_l.
   (* Oh wow, this is annyoing... *)
-  rewrite associative -always_and_sep_r'.
+  rewrite assoc -always_and_sep_r'.
   by rewrite /vs always_elim impl_elim_r.
 Qed.
 
